projects/SmullyanGIT/PA.v
@@ -17,9 +17,13 @@ Module Tarski's_Theorem_for_Arithmetic.
     nat
   .
 
-  Definition Vr_eq_dec : forall x : Vr, forall y : Vr, {x = y} + {x <> y} :=
-    Nat.eq_dec
-  .
+  Lemma Vr_eq_dec :
+    forall x : Vr,
+    forall y : Vr,
+    {x = y} + {x <> y}.
+  Proof.
+    exact Nat.eq_dec.
+  Qed.
 
   Inductive Tm : Set :=
   | ivarTm : forall x : Vr, Tm
@@ -221,20 +225,65 @@ Module Tarski's_Theorem_for_Arithmetic.
 
   Section BasicMetaTheories.
 
+  Local Ltac case_Vr_eq_dec x1 x2 :=
+    let H := fresh "H" in
+    destruct (Vr_eq_dec x1 x2) as [H | H];
+    simpl;
+    [destruct H | try now contradiction H];
+    try now firstorder
+  .
+
+  Local Ltac simpl_Vr_eq_dec :=
+    simpl;
+    repeat (repeat split; intro);
+    match goal with
+    | H : (if Vr_eq_dec ?x1 ?x2 then ?casel else ?caser) = ?rhs |- _ => case_Vr_eq_dec x1 x2
+    | H : ?lhs = (if Vr_eq_dec ?x1 ?x2 then ?casel else ?caser) |- _ => case_Vr_eq_dec x1 x2
+    | |- (if Vr_eq_dec ?x1 ?x2 then ?casel else ?caser) = ?rhs => case_Vr_eq_dec x1 x2
+    | |- ?lhs = (if Vr_eq_dec ?x1 ?x2 then ?casel else ?caser) => case_Vr_eq_dec x1 x2
+    end
+  .
+
+  Lemma in_getFreeVarsTm_iff :
+    forall t : Tm,
+    forall z : Vr,
+    In z (getFreeVarsTm t) <-> occursFreeInTm z t = true.
+  Proof with auto_rewrite.
+    induction t; intros z; simpl...
+    simpl_Vr_eq_dec.
+  Qed.
+
+  Local Hint Resolve in_getFreeVarsTm_iff : core.
+
   Lemma in_getFreeVarsForm_iff :
     forall f : Form,
-    forall x : Vr,
-    In x (getFreeVarsForm f) <-> occursFreeInForm x f = true.
-  Proof with eauto.
-  Admitted.
+    forall z : Vr,
+    In z (getFreeVarsForm f) <-> occursFreeInForm z f = true.
+  Proof with auto_rewrite.
+    induction f; intros z; simpl...
+    all: try (repeat rewrite in_getFreeVarsTm_iff; now firstorder).
+    case_Vr_eq_dec y z.
+  Qed.
 
   Lemma getMaxNumOfFreeVarsInTm_lt_implies :
     forall t : Tm,
     forall x : Vr,
     getMaxNumOfFreeVarsInTm t < x ->
     occursFreeInTm x t = false.
-  Proof with eauto.
-  Admitted.
+  Proof with lia || auto_rewrite.
+    assert ( claim1 :
+      forall z : Vr,
+      forall x : Vr,
+      max z 0 < x ->
+      (if Vr_eq_dec z x then true else false) = false
+    ).
+    { intros z x.
+      case_Vr_eq_dec z x...
+    }
+    unfold getMaxNumOfFreeVarsInTm.
+    induction t; simpl; intros z H...
+    all: rewrite fold_right_max_0_app in H; split; [apply IHt1 | apply IHt2]...
+  Qed.
 
   Lemma evalTm_equiv_if_FVs_equiv :
     forall t : Tm,
@@ -243,7 +292,21 @@ Module Tarski's_Theorem_for_Arithmetic.
     (forall x : Vr, occursFreeInTm x t = true -> E1 x = E2 x) ->
     evalTm E1 t = evalTm E2 t.
   Proof with eauto.
-  Admitted.
+    assert ( claim1 :
+      forall z : Vr,
+      forall E1 : Env,
+      forall E2 : Env,
+      (forall x : Vr, (if Vr_eq_dec z x then true else false) = true -> E1 x = E2 x) ->
+      E1 z = E2 z
+    ).
+    { intros v va1 va2 H.
+      apply H.
+      case_Vr_eq_dec v v...
+    }
+    induction t; simpl...
+    all: intros E1 E2 H; rewrite (IHt1 E1 E2), (IHt2 E1 E2)...
+    all: intros x H0; apply H, orb_true_iff...
+  Qed.
 
   Lemma evalForm_equiv_if_FVs_equiv :
     forall f : Form,
@@ -251,8 +314,31 @@ Module Tarski's_Theorem_for_Arithmetic.
     forall E2 : Env,
     (forall x : Vr, occursFreeInForm x f = true -> E1 x = E2 x) ->
     evalForm E1 f <-> evalForm E2 f.
-  Proof with eauto.
-  Admitted.
+  Proof with tauto || eauto.
+    induction f; simpl; intros E1 E2 H...
+    1, 2: rewrite (evalTm_equiv_if_FVs_equiv t1 E1 E2), (evalTm_equiv_if_FVs_equiv t2 E1 E2)...
+    1, 2, 3, 4: intros x H0; apply H, orb_true_iff...
+    - firstorder.
+    - split; intros H0 H1; [apply (IHf2 E1 E2) | apply (IHf2 E2 E1)].
+      + intros x H2.
+        apply H, orb_true_iff...
+      + apply H0, (IHf1 E2 E1)...
+        intros x H2.
+        symmetry.
+        apply H, orb_true_iff...
+      + intros x H2.
+        symmetry.
+        apply H, orb_true_iff...
+      + apply H0, (IHf1 E1 E2)...
+        intros x H2.
+        apply H, orb_true_iff...
+    - enough (claim1 : forall n : nat, evalForm (fun z : Vr => if Vr_eq_dec y z then n else E1 z) f <->  evalForm (fun z : Vr => if Vr_eq_dec y z then n else E2 z) f) by firstorder.
+      intros n.
+      rewrite (IHf (fun z : Vr => if Vr_eq_dec y z then n else E1 z) (fun z : Vr => if Vr_eq_dec y z then n else E2 z))...
+      simpl_Vr_eq_dec.
+      apply H.
+      simpl_Vr_eq_dec.
+  Qed.
 
   Lemma applySubst_Tm_preserves_evalTm :
     forall t : Tm,
@@ -260,22 +346,65 @@ Module Tarski's_Theorem_for_Arithmetic.
     forall E : Env,
     evalTm (fun z : Vr => evalTm E (applySubst_Vr sigma z)) t = evalTm E (applySubst_Tm sigma t).
   Proof with eauto.
-  Admitted.
+    induction t; simpl...
+  Qed.
 
   Lemma the_main_reason_for_introducing_chi :
     forall f : Form,
     forall sigma : substitution,
     isFreshVarIn_applySubst_Form sigma (chi sigma f) f.
   Proof with eauto.
-  Admitted.
+    assert ( claim1 :
+      forall sigma : substitution,
+      forall f : Form,
+      forall x : Vr,
+      occursFreeInForm x f = true ->
+      occursFreeInTm (chi sigma f) (applySubst_Vr sigma x) = false
+    ).
+    { intros sigma f x H.
+      enough (claim1_aux1 : getMaxNumOfFreeVarsInTm (applySubst_Vr sigma x) < chi sigma f) by now apply getMaxNumOfFreeVarsInTm_lt_implies.
+      unfold chi, fold_right_max_0.
+      enough (claim1_aux2 : fold_right max 0 (map (fun z : Vr => getMaxNumOfFreeVarsInTm (applySubst_Vr sigma z)) (getFreeVarsForm f)) >= getMaxNumOfFreeVarsInTm (applySubst_Vr sigma x)) by lia.
+      rewrite <- in_getFreeVarsForm_iff in H.
+      apply fold_right_max_0_in, in_map_iff...
+    }
+    unfold isFreshVarIn_applySubst_Form.
+    do 2 auto_rewrite.
+    apply claim1, in_getFreeVarsForm_iff...
+  Qed.
 
   Lemma applySubst_Form_preserves_evalForm :
     forall f : Form,
     forall sigma : substitution,
     forall E : Env,
     evalForm (fun z : Vr => evalTm E (applySubst_Vr sigma z)) f <-> evalForm E (applySubst_Form sigma f).
-  Proof with eauto.
-  Admitted.
+  Proof with tauto || eauto.
+    induction f; simpl; intros sigma E.
+    - do 2 rewrite applySubst_Tm_preserves_evalTm...
+    - do 2 rewrite applySubst_Tm_preserves_evalTm...
+    - firstorder.
+    - split; intros H H0; apply IHf2, H, IHf1...
+    - enough (claim1 : forall n : nat, evalForm (fun z : Vr => if Vr_eq_dec y z then n else evalTm E (applySubst_Vr sigma z)) f <-> evalForm (fun z : Vr => if Vr_eq_dec (chi sigma (allF y f)) z then n else E z) (applySubst_Form (consSubst y (ivarTm (chi sigma (allF y f))) sigma) f)) by firstorder.
+      intros n.
+      rewrite <- (IHf (consSubst y (ivarTm (chi sigma (allF y f))) sigma) (fun z : Vr => if Vr_eq_dec (chi sigma (allF y f)) z then n else E z)).
+      apply evalForm_equiv_if_FVs_equiv.
+      intros x H.
+      unfold consSubst, applySubst_Vr.
+      simpl.
+      case_Vr_eq_dec y x.
+      + case_Vr_eq_dec y y.
+        case_Vr_eq_dec (chi sigma (allF y f)) (chi sigma (allF y f)).
+      + case_Vr_eq_dec x y.
+        apply evalTm_equiv_if_FVs_equiv.
+        intros x' H2.
+        simpl_Vr_eq_dec.
+        assert (claim2 : isFreshVarIn_applySubst_Form sigma (chi sigma (allF y f)) (allF y f)) by apply the_main_reason_for_introducing_chi.
+        unfold isFreshVarIn_applySubst_Form in claim2.
+        rewrite forallb_true_iff in claim2.
+        enough (claim3 : negb (occursFreeInTm (chi sigma (allF y f)) (sigma x)) = true) by now rewrite H2 in claim3.
+        apply claim2, in_getFreeVarsForm_iff.
+        simpl_Vr_eq_dec.
+  Qed.
 
   End BasicMetaTheories.
 
